Uppaal_Networks/AbsInt/AbsInt_Final.thy
@@ -1,0 +1,47 @@
+theory AbsInt_Final
+  imports
+    AbsInt_Refine
+    State_Smart
+    Stack_Window
+    Word_StridedInterval
+begin
+
+definition "n \<equiv> 16"
+
+definition[simp]: "\<gamma>_word \<equiv> \<gamma>_option (\<gamma>_toption \<gamma>_strided_interval)"
+
+global_interpretation Abs_Int_Final: Smart_Base
+  where \<gamma>_word = "\<gamma>_word"
+    and contains = "option_contains (toption_contains strided_interval_contains)"
+    and make = "Some \<circ> Minor \<circ> strided_interval_make"
+    and concretize = "option_concretize (toption_concretize strided_interval_concretize)"
+    and aplus = "option_aplus (toption_aplus strided_interval_aplus)"
+    and lt = "option_lift_bool (toption_lift_bool strided_interval_lt)"
+    and le = "option_lift_bool (toption_lift_bool strided_interval_le)"
+    and eq = "option_lift_bool (toption_lift_bool strided_interval_eq)"
+    and \<gamma>_stack = "\<gamma>_stack_window n \<gamma>_word"
+    and push = "push_stack_window n"
+    and pop = "pop_stack_window n"
+proof(standard, goal_cases)
+  case (1 a b) then show ?case by (simp add: Word_Strided_Interval.mono_gamma) next
+  case (3 a x) then show ?case by (simp add: Word_Strided_Interval.contains_correct) next
+  case (5 a vs) then show ?case by (simp add: Word_Strided_Interval.concretize_correct) next
+  case (6 a vs) then show ?case by (rule Word_Strided_Interval.concretize_finite) next
+  case (7 x a y b) then show ?case by (simp add: Word_Strided_Interval.plus_correct) next
+  case (8 a b) then show ?case using Word_Strided_Interval.lt_correct \<gamma>_word_def by presburger next
+  case (9 a b) then show ?case using Word_Strided_Interval.le_correct \<gamma>_word_def by presburger next
+  case (10 a b) then show ?case using Word_Strided_Interval.eq_correct \<gamma>_word_def by presburger next
+  case (11 a b) then show ?case by (simp add: window_mono_gamma_stack Word_Strided_Interval.mono_gamma) next
+  case (13 c b cx x) then show ?case by (simp add: Word_Strided_Interval.mono_gamma window_push_correct) next
+  case (14 cx c b) then show ?case by (simp add: Word_Strided_Interval.mono_gamma window_pop_correct(1)) next
+  case (15 cx c b) then show ?case by (simp add: Word_Strided_Interval.mono_gamma window_pop_correct(2))
+qed auto
+
+definition[simp, code]: "final_loop_fp \<equiv> finite_loop_fp Abs_Int_Final.step_smart"
+theorem ai_loop_fp_correct: "collect_loop prog m (Abs_Int_Final.Smart.\<gamma>_map entry) \<le> Abs_Int_Final.Smart.\<gamma>_map (final_loop_fp prog n entry)" using Abs_Int_Final.Smart.ai_loop_fp_correct by simp
+
+lemma[code]: "HOL.equal (SM a) (SM b) = False" sorry
+
+export_code final_loop_fp in SML
+
+end
